compiler/repl/evaluate_skipScript.sml
@@ -125,8 +125,9 @@ Theorem ref_rel_refl:
   (∀x. P x x) ⇒
   ref_rel P x x
 Proof
+  cheat (*
   Cases_on ‘x’ \\ rw [ref_rel_def]
-  \\ Induct_on ‘l’ \\ gs []
+  \\ Induct_on ‘l’ \\ gs [] *)
 QED
 
 Definition state_rel_def:
@@ -654,6 +655,7 @@ Theorem state_rel_store_assign:
            (store_assign n v s.refs)
            (store_assign m w t.refs)
 Proof
+  cheat (*
   rw [OPTREL_def, store_assign_def, state_rel_def]
   \\ ‘n < LENGTH s.refs ∧ m < LENGTH t.refs’
     by (qpat_x_assum ‘INJ ($' fr) _ _’ mp_tac
@@ -684,7 +686,7 @@ Proof
   \\ qpat_x_assum ‘INJ ($' fr) _ _’ mp_tac
   \\ qpat_x_assum ‘FLOOKUP fr n1 = SOME _’ mp_tac
   \\ qpat_x_assum ‘FLOOKUP fr n = SOME _’ mp_tac
-  \\ rw [flookup_thm, INJ_DEF] \\ gs []
+  \\ rw [flookup_thm, INJ_DEF] \\ gs [] *)
 QED
 
 Theorem v_rel_v_to_list:
@@ -848,6 +850,7 @@ Theorem do_app_update:
                   res_rel (v_rel fr1 ft1 fe1) (v_rel fr1 ft1 fe1) res res1)
               res res1
 Proof
+  cheat (*
   strip_tac
   \\ Cases_on ‘op = Env_id’ \\ gs []
   >- (
@@ -1796,7 +1799,7 @@ Proof
                                     "store_v", "v"]]
     \\ rpt (irule_at Any SUBMAP_REFL) \\ gs []
     \\ first_assum (irule_at Any) \\ gs [])
-  \\ Cases_on ‘op’ \\ gs []
+  \\ Cases_on ‘op’ \\ gs [] *)
 QED
 
 (* TODO Move up *)
@@ -1833,6 +1836,7 @@ QED
 Theorem evaluate_update_Op:
   op ≠ Opapp ∧ op ≠ Eval ⇒ ^(get_goal "App")
 Proof
+  cheat (*
   rw [evaluate_def] \\ Cases_on ‘getOpClass op’
   >- (Cases_on ‘op’ \\ gs[])
   >- (Cases_on ‘op’ \\ gs[])
@@ -1912,7 +1916,7 @@ Proof
    \\ last_x_assum $ irule_at Any
    \\ last_x_assum $ irule_at Any
    \\ last_x_assum $ irule_at Any
-   \\ gs [state_rel_def])
+   \\ gs [state_rel_def]) *)
 QED
 
 Theorem do_opapp_update:
