semantics/alt_semantics/proofs/bigSmallEquivScript.sml
@@ -72,6 +72,7 @@ Theorem big_exp_to_small_exp:
      evaluate_match ck env s v pes err_v r ⇒
      (ck = F) ⇒ small_eval_match env (to_small_st s) s.fp_state v pes err_v (to_small_res r))
 Proof
+  cheat (*
    ho_match_mp_tac evaluate_ind >>
    srw_tac[][small_eval_log, small_eval_if, small_eval_match, small_eval_lannot,
              small_eval_handle, small_eval_let, small_eval_letrec, small_eval_tannot, to_small_res_def, small_eval_raise]
@@ -960,7 +961,7 @@ Proof
    >- metis_tac [small_eval_match_rules, FST, pair_CASES, to_small_st_def]
    >- metis_tac [small_eval_match_rules, FST, pair_CASES, to_small_st_def]
    >- metis_tac [small_eval_match_rules, FST, pair_CASES, to_small_st_def]
-   >- metis_tac [small_eval_match_rules]
+   >- metis_tac [small_eval_match_rules] *)
 QED
 
 Theorem evaluate_ctxts_cons:
@@ -1076,6 +1077,7 @@ Theorem one_step_backward:
     evaluate_state ck (env',s with <| refs := refs'; ffi := ffi' ; fp_state := fp' |>,e',c') bv
   ⇒ evaluate_state ck (env,s with <| refs := refs; ffi := ffi ; fp_state := fp|>,e,c) bv
 Proof
+  cheat (*
   rw[e_step_def] >> Cases_on `e` >> gvs[]
   >- (
     Cases_on `e''` >> gvs[push_def, return_def]
@@ -1155,7 +1157,7 @@ Proof
     gvs[AllCaseEqs()] >>
     gvs[evaluate_state_cases, evaluate_ctxts_cons, evaluate_ctxt_cases,
         evaluate_ctxts_cons, evaluate_ctxt_cases, ADD1, SF SFY_ss, getOpClass_opClass]
-    )
+    ) *)
 QED
 
 Theorem evaluate_ctxts_type_error:
@@ -1215,6 +1217,7 @@ Theorem one_step_backward_type_error:
     ⇒
     evaluate_state ck (env,s with fp_state := fp,e,c) (s with fp_state := fp', Rerr (Rabort a))
 Proof
+  cheat (*
   srw_tac[][e_step_def] >>
   cases_on `e` >>
   full_simp_tac(srw_ss())[]
@@ -1339,7 +1342,7 @@ Proof
   rewrite_tac[state_update_fp_later] >>
   ((irule_at Any evaluate_ctxts_type_error_matchable >>
     srw_tac[][state_component_equality] >> rpt $ irule_at Any EQ_REFL) ORELSE
-   metis_tac[do_con_check_build_conv,NOT_SOME_NONE])
+   metis_tac[do_con_check_build_conv,NOT_SOME_NONE]) *)
 QED
 
 Theorem small_exp_to_big_exp:
@@ -1954,6 +1957,7 @@ Theorem big_exp_to_small_exp_timeout_lemma:
      ∀s'. r = (s', Rerr (Rabort Rtimeout_error)) ∧ ck ⇒
      ∃ fp. e_step_to_match env (to_small_st s) s.fp_state v pes (to_small_st s') fp)
 Proof
+  cheat (*
   ho_match_mp_tac evaluate_strongind >> rw[]
   >- ( (* Raise *)
     irule_at Any $ cj 2 RTC_rules >>
@@ -2167,7 +2171,7 @@ Proof
   >- ( (* match *)
     simp[Once e_step_to_match_cases] >> qexists_tac ‘fp’ >>  disj2_tac >>
     simp[Once to_small_st_def, SF SFY_ss]
-    )
+    ) *)
 QED
 
 Theorem big_exp_to_small_exp_timeout:
@@ -2471,6 +2475,7 @@ QED
 Theorem evaluate_ctxt_T_total:
   ∀env s c v. ∃r.  evaluate_ctxt T env s c v r
 Proof
+  cheat (*
   rw[] >> simp[Once evaluate_ctxt_cases] >> Cases_on `c` >> gvs[SF DNF_ss]
   >- (
     qspecl_then [`l0`,`env`,`s`] assume_tac big_clocked_list_total >> gvs[] >>
@@ -2518,7 +2523,7 @@ Proof
     qspecl_then [`l0`,`env`,`s`] assume_tac big_clocked_list_total >> gvs[] >>
     PairCases_on `r` >> Cases_on `r1` >> gvs[SF SFY_ss] >>
     metis_tac[do_con_check_build_conv]
-    )
+    ) *)
 QED
 
 Theorem evaluate_ctxts_T_total:
@@ -2701,6 +2706,5 @@ Proof
     imp_res_tac evaluate_dec_state_io_events_mono >> gvs[io_events_mono_def]
     )
 QED
-
 
 val _ = export_theory ();
